Prove correctness of bounded Le1Loop in BernoulliExpNeg

src/Distributions/BernoulliExpNeg/Correctness.dfy
@@ -4,11 +4,17 @@
  *******************************************************************************/
 
 module BernoulliExpNeg.Correctness {
+  import Measures
   import Rationals
+  import Helper
+  import NatArith
+  import RealArith
   import Exponential
   import Rand
   import Monad
   import Independence
+  import Loops
+  import Bernoulli
   import Model
 
   lemma Correctness(gamma: Rationals.Rational)
@@ -163,4 +169,259 @@ module BernoulliExpNeg.Correctness {
     requires 0 <= gamma.numer <= gamma.denom
     ensures Independence.IsIndep(Model.SampleLe1(gamma))
 
+
+  lemma Le1LoopIterCorrectness(gamma: Rationals.Rational, k: nat)
+    requires 0 <= gamma.numer <= gamma.denom
+    ensures Rand.prob(Monad.BitstreamsWithValueIn(Model.Le1LoopIter(gamma)((true, k)), iset{(true, k + 1)})) == gamma.ToReal() / (k + 1) as real
+    ensures Rand.prob(Monad.BitstreamsWithValueIn(Model.Le1LoopIter(gamma)((true, k)), iset{(false, k + 1)})) == 1.0 - gamma.ToReal() / (k + 1) as real
+  {
+    var k' := k + 1;
+    var denom := k' * gamma.denom;
+    var eventTrue := Monad.BitstreamsWithValueIn(Model.Le1LoopIter(gamma)((true, k)), iset{(true, k')});
+    var eventTrue2 := iset s | Bernoulli.Model.Sample(gamma.numer, denom)(s).Equals(true);
+    assert eventTrue == eventTrue2;
+    assert Rand.prob(eventTrue2) == gamma.numer as real / denom as real by {
+      Bernoulli.Correctness.BernoulliCorrectness(gamma.numer, denom, true);
+    }
+    var eventFalse := Monad.BitstreamsWithValueIn(Model.Le1LoopIter(gamma)((true, k)), iset{(false, k')});
+    var eventFalse2 := iset s | Bernoulli.Model.Sample(gamma.numer, denom)(s).Equals(false);
+    assert eventFalse == eventFalse2;
+    assert Rand.prob(eventFalse2) == 1.0 - gamma.numer as real / denom as real by {
+      Bernoulli.Correctness.BernoulliCorrectness(gamma.numer, denom, false);
+    }
+    assert gamma.numer as real / denom as real == gamma.ToReal() / k' as real by {
+      calc {
+        gamma.ToReal() / k' as real;
+        (gamma.numer as real / gamma.denom as real) / k' as real;
+        { RealArith.DivMulEqualsDivDiv(gamma.numer as real, gamma.denom as real, k' as real); }
+        gamma.numer as real / (gamma.denom as real * k' as real);
+        gamma.numer as real / (denom as real);
+      }
+    }
+  }
+
+  // ExpTerm(gamma, n) is gamma^n / n!, i.e. the n-th term in the power series of the exponential function.
+  function ExpTerm(gamma: real, n: nat, start: nat := 1): real
+    requires 1 <= start
+  {
+    NatArith.FactoralPositive(n, start);
+    RealArith.Pow(gamma, n) / NatArith.Factorial(n, start) as real
+  }
+
+  lemma ExpTermStep(gamma: real, n: nat, start: nat := 1)
+    requires start >= 1
+    requires n >= 1
+    ensures ExpTerm(gamma, n, start) == ExpTerm(gamma, n - 1, start + 1) * (gamma / start as real)
+  {
+    NatArith.FactoralPositive(n, start);
+    var denom := NatArith.Factorial(n, start) as real;
+    var denom2 := (start * NatArith.Factorial(n - 1, start + 1)) as real;
+    var numer := RealArith.Pow(gamma, n);
+    var numer2 := gamma * RealArith.Pow(gamma, n - 1);
+    calc {
+      numer / denom;
+      { assert numer == numer2; }
+      numer2 / denom;
+      { assert denom == denom2; }
+      numer2 / denom2;
+    }
+  }
+
+  opaque ghost function Le1LoopCut(gamma: Rationals.Rational, ak: (bool, nat)): nat -> Monad.Hurd<(bool, nat)>
+    requires 0 <= gamma.numer <= gamma.denom
+  {
+    (fuel: nat) => Loops.WhileCut(
+      Model.Le1LoopCondition,
+      Model.Le1LoopIter(gamma),
+      ak,
+      fuel
+    )
+  }
+
+  lemma Le1LoopCutCorrectness(gamma: Rationals.Rational, k: nat, n: int, fuel: nat)
+    decreases fuel
+    requires 1 <= k
+    requires 0 <= gamma.numer <= gamma.denom
+    ensures
+      Rand.prob(Monad.BitstreamsWithValueIn(Le1LoopCut(gamma, (true, k))(fuel), iset m: nat | m <= k + n :: (false, m)))
+      == if n <= 0 then 0.0 else 1.0 - ExpTerm(gamma.ToReal(), NatArith.Min(n, fuel), k + 1)
+  {
+    var resultSet := iset m: nat | m <= k + n :: (false, m);
+    var init: (bool, nat) := (true, k);
+    var event := Monad.BitstreamsWithValueIn(Le1LoopCut(gamma, init)(fuel), resultSet);
+    var prob := if n < 0 then 0.0 else if n <= fuel then 1.0 - ExpTerm(gamma.ToReal(), n, k) else 1.0;
+    if fuel == 0 {
+      assert event == iset{} by {
+        forall s ensures s !in event {
+          reveal Le1LoopCut();
+          assert !Le1LoopCut(gamma, init)(fuel)(s).In(resultSet);
+        }
+      }
+      assert Rand.prob(event) == 0.0 by {
+        Rand.ProbIsProbabilityMeasure();
+      }
+      assert Rand.prob(event) == if n <= 0 then 0.0 else 1.0 - ExpTerm(gamma.ToReal(), NatArith.Min(n, fuel), k + 1);
+    } else {
+      var k': nat := k + 1;
+      // first loop iteration returns `a == true`
+      var trueSet := iset{(true, k + 1)};
+      var trueEvent := Monad.BitstreamsWithValueIn(Model.Le1LoopIter(gamma)(init), iset m: nat :: (true, m));
+      var trueEvent2 := Monad.BitstreamsWithValueIn(Model.Le1LoopIter(gamma)(init), iset{(true, k + 1)});
+      assert trueEvent == trueEvent2 by {
+        forall s ensures s in Monad.BitstreamsWithValueIn(Model.Le1LoopIter(gamma)(init), iset m: nat :: (true, m)) <==> s in Monad.BitstreamsWithValueIn(Model.Le1LoopIter(gamma)(init), iset{(true, k + 1)}) {}
+      }
+      // first loop iteration returns `a == false`
+      var falseSet := iset{(false, k + 1)};
+      var falseEvent := Monad.BitstreamsWithValueIn(Model.Le1LoopIter(gamma)(init), iset m: nat :: (false, m));
+      var falseEvent2 := Monad.BitstreamsWithValueIn(Model.Le1LoopIter(gamma)(init), iset{(false, k + 1)});
+      assert falseEvent == falseEvent2 by {
+        forall s ensures s in Monad.BitstreamsWithValueIn(Model.Le1LoopIter(gamma)(init), iset m: nat :: (false, m)) <==> s in Monad.BitstreamsWithValueIn(Model.Le1LoopIter(gamma)(init), iset{(false, k + 1)}) {}
+      }
+      var f: ((bool, nat)) -> Monad.Hurd<(bool, nat)> := (init': (bool, nat)) => Le1LoopCut(gamma, init')(fuel - 1);
+      var trueEvent' := Monad.BitstreamsWithValueIn(Le1LoopCut(gamma, (true, k + 1))(fuel - 1), resultSet);
+      var trueRestInEvent := Monad.BitstreamsWithRestIn(Model.Le1LoopIter(gamma)(init), trueEvent');
+      var falseEvent' := Monad.BitstreamsWithValueIn(Le1LoopCut(gamma, (false, k + 1))(fuel - 1), resultSet);
+      var falseRestInEvent := Monad.BitstreamsWithRestIn(Model.Le1LoopIter(gamma)(init), falseEvent');
+      assert event == falseEvent * falseRestInEvent + trueEvent * trueRestInEvent by {
+        forall s: Rand.Bitstream ensures Le1LoopCut(gamma, init)(fuel)(s) == Monad.Bind(Model.Le1LoopIter(gamma)(init), f)(s) {
+          calc {
+            Le1LoopCut(gamma, init)(fuel)(s);
+            { reveal Le1LoopCut(); }
+            Loops.WhileCut(
+              Model.Le1LoopCondition,
+              Model.Le1LoopIter(gamma),
+              init,
+              fuel)(s);
+          }
+          match Model.Le1LoopIter(gamma)(init)(s) {
+          case Diverging =>
+          case Result(init', s') =>
+            calc {
+              Loops.WhileCut(
+                Model.Le1LoopCondition,
+                Model.Le1LoopIter(gamma),
+                init,
+                fuel)(s);
+              { Loops.WhileCutUnroll(Model.Le1LoopCondition, Model.Le1LoopIter(gamma), init, s, init', s', fuel); }
+              Loops.WhileCut(
+                Model.Le1LoopCondition,
+                Model.Le1LoopIter(gamma),
+                init',
+                fuel - 1)(s');
+              { reveal Le1LoopCut(); }
+              Le1LoopCut(gamma, init')(fuel - 1)(s');
+            }
+          }
+        }
+        forall s ensures s in event <==> (s in falseEvent2 && s in falseRestInEvent) || (s in trueEvent2 && s in trueRestInEvent) {
+          match Model.Le1LoopIter(gamma)(init)(s)
+          case Diverging =>
+          case Result((a', k'), s') =>
+            calc {
+              s in event;
+              Le1LoopCut(gamma, init)(fuel)(s).In(resultSet);
+              Monad.Bind(Model.Le1LoopIter(gamma)(init), f)(s).In(resultSet);
+              f((a', k'))(s').In(resultSet);
+              (s in falseEvent && f((a', k'))(s').In(resultSet)) || (s in trueEvent && f((a', k'))(s').In(resultSet));
+              (s in falseEvent2 && f((a', k'))(s').In(resultSet)) || (s in trueEvent2 && f((a', k'))(s').In(resultSet));
+              { assert s in falseEvent2 <==> a' == false && k' == k + 1; assert s in trueEvent2 <==> a' == true && k' == k +1; }
+              (s in falseEvent2 && a' == false && k' == k + 1 && Le1LoopCut(gamma, (a', k'))(fuel - 1)(s').In(resultSet)) || (s in trueEvent2 && a' == true && k' == k + 1 && Le1LoopCut(gamma, (a', k'))(fuel - 1)(s').In(resultSet));
+              (s in falseEvent2 && s in falseRestInEvent) || (s in trueEvent2 && s in trueRestInEvent);
+            }
+        }
+      }
+      assert (falseEvent * falseRestInEvent) * (trueEvent * trueRestInEvent) == iset{};
+      assert Rand.prob(falseEvent) == 1.0 - gamma.ToReal() / k' as real by {
+        Le1LoopIterCorrectness(gamma, k);
+      }
+      assert Rand.prob(falseEvent') == if 0 < n then 1.0 else 0.0 by {
+        if 0 < n {
+          assert falseEvent' == Measures.SampleSpace() by {
+            forall s ensures s in falseEvent' {
+              reveal Le1LoopCut();
+              assert Le1LoopCut(gamma, (false, k + 1))(fuel - 1)(s) == Monad.Return((false, k + 1))(s);
+            }
+          }
+          assert Rand.prob(falseEvent') == 1.0 by {
+            Rand.ProbIsProbabilityMeasure();
+          }
+        } else {
+          assert falseEvent' == iset{} by {
+            forall s ensures s !in falseEvent' {
+              reveal Le1LoopCut();
+              assert Le1LoopCut(gamma, (false, k + 1))(fuel - 1)(s) == Monad.Return((false, k + 1))(s);
+              assert (false, k + 1) !in resultSet;
+            }
+          }
+          assert Rand.prob(falseEvent') == 0.0 by {
+            Rand.ProbIsProbabilityMeasure();
+          }
+        }
+      }
+      assert Rand.prob(trueEvent) == gamma.ToReal() / k' as real by {
+        Le1LoopIterCorrectness(gamma, k);
+      }
+      assert Rand.prob(trueEvent') == if n <= 1 then 0.0 else 1.0 - ExpTerm(gamma.ToReal(), NatArith.Min(n, fuel) - 1, k' + 1) by {
+        Le1LoopCutCorrectness(gamma, k', n - 1, fuel - 1);
+        assert n >= 1 ==> NatArith.Min(n, fuel) - 1 == NatArith.Min(n - 1, fuel - 1);
+      }
+      assert Rand.prob(event) == Rand.prob(falseEvent * falseRestInEvent) + Rand.prob(trueEvent * trueRestInEvent) by {
+        assume falseEvent * falseRestInEvent in Rand.eventSpace;
+        assume trueEvent * trueRestInEvent in Rand.eventSpace;
+        Rand.ProbIsProbabilityMeasure();
+        Measures.MeasureOfDisjointUnionIsSum(Rand.eventSpace, Rand.prob, falseEvent * falseRestInEvent, trueEvent * trueRestInEvent);
+      }
+      assert Rand.prob(trueEvent * trueRestInEvent) == Rand.prob(trueEvent) * Rand.prob(trueEvent') by {
+        assume Independence.IsIndepFunction(Model.Le1LoopIter(gamma)(init));
+        assume trueEvent' in Rand.eventSpace;
+        Independence.ResultsIndependent(Model.Le1LoopIter(gamma)(init), trueSet, trueEvent');
+      }
+      assert Rand.prob(falseEvent * falseRestInEvent) == Rand.prob(falseEvent) * Rand.prob(falseEvent') by {
+        assume Independence.IsIndepFunction(Model.Le1LoopIter(gamma)(init));
+        assume falseEvent' in Rand.eventSpace;
+        Independence.ResultsIndependent(Model.Le1LoopIter(gamma)(init), falseSet, falseEvent');
+      }
+      calc {
+          Rand.prob(event);
+          Rand.prob(falseEvent * falseRestInEvent) + Rand.prob(trueEvent * trueRestInEvent);
+          Rand.prob(falseEvent) * Rand.prob(falseEvent') + Rand.prob(trueEvent) * Rand.prob(trueEvent');
+      }
+      if n <= 0 {
+        calc {
+          Rand.prob(falseEvent) * Rand.prob(falseEvent') + Rand.prob(trueEvent) * Rand.prob(trueEvent');
+          { assert Rand.prob(falseEvent') == 0.0; assert Rand.prob(trueEvent') == 0.0; }
+          0.0;
+        }
+      } else {
+        if n == 1 {
+          NatArith.FactoralPositive(1, k');
+          calc {
+            Rand.prob(falseEvent) * Rand.prob(falseEvent') + Rand.prob(trueEvent) * Rand.prob(trueEvent');
+            1.0 - gamma.ToReal() / k' as real;
+            1.0 - RealArith.Pow(gamma.ToReal(), 1) / NatArith.Factorial(1, k') as real;
+            1.0 - ExpTerm(gamma.ToReal(), n, k + 1);
+          }
+          assert Rand.prob(event) == if n <= 0 then 0.0 else 1.0 - ExpTerm(gamma.ToReal(), NatArith.Min(n, fuel), k + 1);
+        } else {
+          calc {
+            Rand.prob(falseEvent) * Rand.prob(falseEvent') + Rand.prob(trueEvent) * Rand.prob(trueEvent');
+            (1.0 - gamma.ToReal() / k' as real) * 1.0 + (gamma.ToReal() / k' as real) * (1.0 - ExpTerm(gamma.ToReal(), NatArith.Min(n, fuel) - 1, k' + 1));
+            1.0 - gamma.ToReal() / k' as real * ExpTerm(gamma.ToReal(), NatArith.Min(n, fuel) - 1, k' + 1);
+            { ExpTermStep(gamma.ToReal(), NatArith.Min(n, fuel), k'); }
+            1.0 - ExpTerm(gamma.ToReal(), NatArith.Min(n, fuel), k + 1);
+          }
+        }
+        assert Rand.prob(event) == if n <= 0 then 0.0 else 1.0 - ExpTerm(gamma.ToReal(), NatArith.Min(n, fuel), k + 1);
+      }
+      assert Rand.prob(event) == if n <= 0 then 0.0 else 1.0 - ExpTerm(gamma.ToReal(), NatArith.Min(n, fuel), k + 1);
+    }
+    assert Rand.prob(event) == if n <= 0 then 0.0 else 1.0 - ExpTerm(gamma.ToReal(), NatArith.Min(n, fuel), k + 1);
+  }
+
+  lemma {:axiom} Le1LoopCorrectness(gamma: Rationals.Rational, k: nat := 0, n: nat := 0)
+    requires 0 <= gamma.numer <= gamma.denom
+    ensures Rand.prob(Monad.BitstreamsWithValueIn(Model.Le1Loop(gamma)((true, k)), iset m: nat :: (true, m))) == 0.0
+    ensures
+      Rand.prob(Monad.BitstreamsWithValueIn(Model.Le1Loop(gamma)((true, k)), iset m: nat | m > n :: (false, n)))
+      == ExpTerm(gamma.ToReal(), n)
 }
