src/Math/NatArith.dfy
@@ -7,5 +7,14 @@ module NatArith {
     if a < b then a else b
   }
 
+  function Factorial(n: nat, start: nat := 1): nat {
+    if n == 0 then 1 else start * Factorial(n - 1, start + 1)
+  }
+
+  lemma FactoralPositive(n: nat, start: nat := 1)
+    requires start >= 1
+    ensures Factorial(n, start) >= 1
+  {}
+
   // TODO: a lot of functions from the helper module should go here.
 }
